.

Instructor/Lectures/lecture_03_04.lean
@@ -30,7 +30,7 @@ def id_bool : Bool → Bool
 ## Functions varying in argument types
 
 Beyond having different names, these
-functions *vary* only in the types of
+functions vary only in the types of
 their argument and return values. 
 
 We wouldn't want to have to write one
@@ -41,7 +41,7 @@ definition into a parameter (argument).
 -/
 
 /-!
-## Factor out variability into a type parameter
+## Abstract type variabilities as parameters
 
 If we bind a name, such as *T* or *α* ,to
 a first *type* argument, then we can define
@@ -82,7 +82,7 @@ function for any type of value.
 #eval id_poly Bool true
 
 /-!
-## Parametric Polymorphism
+### Parametric Polymorphism
 
 What we're seeing here is called parametric polymorphism! We have 
 one function definition that can take arguments of many different 
@@ -97,7 +97,7 @@ will report an error. Let's try.
 #check id_poly Bool 7   -- Lean says it can't convert 7 into a Bool
 
 /-!
-# Implicit Arguments
+### Implicit Arguments
 
 You might have noticed that in principle Lean can always infer
 the *type value* of the first argument to the id_poly function
@@ -134,4 +134,173 @@ be returned.
 #eval id_poly' "Hello!"
 #eval id_poly' true
 
+/-!
+## Polymorphic Higher Order Functions
 
+This is getting cosmic!
+
+## An apply2 function for Natty values
+
+Let's start with some high-order but not
+polymorphic functions. Each one takes a given
+function, f, e.g., from Nat → Nat, along with a
+second argument, a, that serves as an argument to 
+the first argument function. The result will be of
+that same type, e.g., Nat. In particular, the value 
+our function returns must be the result of applying
+f to a *twice*.
+
+As an example, if f is the function that increments
+a natural number a, the result of "applying it twice" 
+to 0 is *increment (increment 0)*. The inner expression
+reduces to 1, then the partially reduced expression,
+increment 1, reduces to 2; and that's the result.
+
+We'll start by writing a function, •apply_twice_nat*,
+that takes a function, *f : Nat → Nat*, and a second
+argument, *a : Nat*, and that returns a result of type
+Nat computed by applying f to the result of applying f
+to a. That's what we mean by *apply2): *f (f a)*. Here
+is a *formal* definition.
+-/
+
+--                         f         a
+def apply2_nat : (Nat → Nat) → Nat → Nat
+| f, a => f (f a)
+
+/-!
+Let's apply this function to some arguments to see 
+what we get. First we need some specific function,
+f, taking and returning a Nat. The Nat.succ function
+will work. This is the *successor* function, which
+returns 1 more than any natural number given as an
+argument. 
+-/
+
+#eval Nat.succ 0    -- 1
+#eval Nat.succ 1    -- 2
+#eval Nat.succ 2    -- 3
+
+#check (Nat.succ)   -- Nat → Nat
+
+/-!
+In addition to such a function we need a natural 
+number as a second argument to apply2_nat. The natural
+number 0 will do just fine. Now that we have values of
+the argument types we can apply the functionto them to
+compute a result.
+
+What do we expect as the result of apppling apply2_nat
+to Nat.succ (of type Nat → Nat) and 0 (of type Nat)? We
+expect it to return the result of applying that function
+to the result of applying that function to 0. The result
+of applying that function to 0 is 1. The result of then
+applying that it to 1 is 2. That is what we expect as a 
+result!
+-/
+
+#eval apply2_nat Nat.succ 0
+
+/-!
+Yay, it seems to work. It gets more interesting when we
+see that we can use *any* function of type Nat → Nat as
+a first argument to this function.  Here are a few little
+puzzles for you to complete by defining simple functions.
+
+First, define a function, *double : Nat → Nat* that 
+returns twice the argument to which it's applied. So for
+example, *double 4* should reduce to *8*.
+-/
+
+def double : Nat → Nat
+| _ => _
+
+#eval apply2_nat double 4     -- expect 16 (2 * (2 * 4))
+#eval apply2_nat double 10    -- expect 40 (2 * (2 * 10))
+
+/-!
+Second, define a function, *square : Nat → Nat*, that 
+reduces to its argument value squared. Then check to see
+that apply2_nat works when you give square as the first
+argument? For example squaring 5 gives 25, and squaring 25 
+gives 625, so apply2_nat square 5 should reduce to 625. 
+Write both the function definition and test cases for a 
+few inputs, including 5. Give your answer here:
+
+#A. define the *square* function here:
+-/
+
+-- here:
+
+/-!
+Write test cases for apply2_nat square for several values,
+including 5, and use them to develop confidence that your
+function definition appears to be working more generally.
+-/
+
+-- here:
+
+/-! 
+### Generalizing from Nat to and type, α
+
+Now if you think about it, we should be able to
+write an apply2 function that does the analogous
+thing but with Stringy things. Given a function, f, 
+from String to String, and an argument, a : String,
+we can always compute *f (f a )*. 
+
+Your new puzzle is to write apply2_string; then give
+examples of applying this function to two different 
+function arguments, and for each of those, to several
+string argument values.
+
+You can make up your own String → String functions.
+For example, a function, exclaim : String → String,
+applied to a string, s, could (append s "!"). There
+is a notation for this: *s ++ "!"*. 
+
+Now you can use this function, exclaimm as a first
+argument to apply2_string. The result is a function
+that is waiting for an argument, s, and that then
+returns returns the result of applying the "baked 
+in") function, f, to s, to compute (f s), and then 
+applies f to that value, for the second time. The
+result is the value of *f (f s))*.  
+
+Show that you can write the programs analogous
+to the corresponding ones for Natty things but
+now for Stringy things, while writing demo and
+test cases. Key idea: A test case defines some
+value to be computed *and* an expected result.
+The passing or failure of a test case reflects
+the consistency of expected and compute value.
+
+## Let's Go Poly!
+
+At this point it should be clear, by analogy
+with earlier material, that we can generalize
+over the specific Nat and String types in the
+previous examples to a general type: call it α!
+Replace the _ here with the *rest of the type*
+of the apply2 function, given that we alrady
+have a specific type in hand, such as String
+or Nat, to which we've bound α. You can now
+use α to specify the rest of the type of the
+function.  
+-/
+
+def apply2 (α : Type) : _
+| f, a => f (f a)
+
+
+#eval apply2 Nat Nat.succ 0   -- expect 2
+#eval apply2 Nat double 1     -- expect 4
+#eval apply2 Nat square 2     -- expect 16
+#eval apply2                  -- expect "Hello!" 
+  String 
+  exclaim 
+  "Hello" 
+
+/-!
+-/
+## Type Inference
